src/proof/hashtriemap/hashtriemap.v
@@ -1,3 +1,7 @@
+From iris.program_logic Require Import atomic.
+From iris.bi.lib Require Import atomic.
+From Perennial.program_logic Require Import atomic.
+
 From New.generatedproof.hashtriemap Require Import hashtriemap.
 From New.proof.hashtriemap Require Import aux.
 From New.proof.hashtriemap Require Import prelude.
@@ -5,6 +9,7 @@ From New.proof.hashtriemap Require Import model.
 
 From New.proof Require Import sync.
 From New.proof.sync Require Import atomic.
+From Perennial.program_logic Require Import atomic.
 
 From iris.base_logic.lib Require Import invariants.
 From iris.proofmode Require Import proofmode.
@@ -13,21 +18,305 @@ From New.golang.theory Require Import struct.
 (* From Perennial.goose_lang.lib Require Import atomic. *)
 From Perennial.algebra Require Import auth_map ghost_var.
 
+Require Import Corelib.Classes.RelationClasses.
+(* From Perennial.goose_lang.lib Require Import atomic. *)
+
 Open Scope Z_scope.
 
 Section proof.
   Context `{hG: heapGS Σ, !invGS Σ, !ffi_semantics _ _}
-    `{(* !mapG Σ w64 w64, !ghost_varG Σ (gmap w64 w64),  *)!ghost_varG Σ bool}
+    `{!ghost_varG Σ bool}
     `{!ghost_varG Σ (gmap w64 w64)}
     `{!mapG Σ w64 w64}
     `{!mapG Σ Z (gmap w64 w64)}
-           `{!globalsGS Σ} {go_ctx: GoContext}.
+    `{!globalsGS Σ} {go_ctx: GoContext}.
 
   Definition map_get `{!IntoVal V} `{!IntoValTyped V t} (v: option V) : V * bool :=
     (default (default_val V) v, bool_decide (is_Some v)).
 
   #[global] Instance : IsPkgInit hashtriemap := define_is_pkg_init True%I.
   #[global] Instance : GetIsPkgInitWf hashtriemap := build_get_is_pkg_init_wf.
+
+  Lemma next_nibble_eq (key: w64) (path: path) :
+    let h := uint.Z (hash_key key) in
+    let n := w64_word_instance.(word.and)
+                                 (w64_word_instance.(word.sru) (hash_key key)
+                                                      (w64_word_instance.(word.sub) (W64 (sh path)) (W64 4)))
+                                 (W64 15) in
+    length path < 16 → uint.Z n = Z.land (h ≫ (sh path - 4)) 15.
+  Proof.
+    intros.
+    unfold h.
+    rewrite word.unsigned_and_nowrap.
+    rewrite word.unsigned_sru.
+    - rewrite word.unsigned_sub.
+      f_equiv; [|word].
+      unfold sh.
+      rewrite wrap_small; auto.
+      + f_equiv.
+        unfold sh. word.
+      + replace (uint.Z (W64 (64 - 4 * length path))) with (64 - 4 * length path) by word.
+        replace (uint.Z (W64 4)) with 4 by word.
+        replace (w64_word_instance_ok.(word.wrap) (64 - 4 * length path - 4)) with (64 - 4 * length path - 4) by word.
+        unfold sh in *.
+        have Hx : ((64 - 4 * length path - 4)) ≥ 0 by lia.
+        have Hrng : 0 ≤ uint.Z (hash_key key) < 2^64 by word.
+        split.
+        * apply Z.shiftr_nonneg. lia.
+        * destruct Hrng as [_ Hrng].
+          apply (Z.le_lt_trans _ (uint.Z (hash_key key))); [|exact Hrng].
+          set x := uint.Z (hash_key key).
+          rewrite Z.shiftr_div_pow2; [|word].
+          apply Z.div_le_upper_bound; [word|].
+          set z := 2 ^ (64 - 4 * length path - 4).
+          have Hz : 1 ≤ z.
+          {
+            replace 1 with (2^0) by lia.
+            apply Z.pow_le_mono_r; lia.
+          }
+          replace (z * x) with (x * z) by lia.
+          clear Hx.
+          have Hx : 0 ≤ x by word.
+          have Hy : 1 ≤ z by lia.
+          have : x * 1 ≤ x * z.
+          { apply (Z.mul_le_mono_nonneg_l _ _ _ Hx).
+            exact Hy. }
+          word.
+    - replace (w64_word_instance.(word.sub) (W64 (sh path)) (W64 4)) with (W64 (sh path - 4)) by word.
+      unfold sh.
+      replace (uint.Z (W64 (64 - 4 * length path - 4))) with (64 - 4 * length path - 4) by word.
+      word.
+  Qed.
+
+  Lemma wp_node__entry (n: loc) (e: loc) :
+    {{{ is_pkg_init hashtriemap ∗
+        n ↦s[hashtriemap.node :: "isEntry"]□ true ∗
+        n ↦s[hashtriemap.node :: "ent"]□ e }}}
+      n @ (ptrT.id hashtriemap.node.id) @ "entry" #()
+      {{{ RET #e; True }}}.
+  Proof.
+    wp_start as "(His_entry & Hent)".
+    wp_auto.
+    wp_finish.
+  Qed.
+
+  Lemma wp_node__indirect (n: loc) (i: loc) :
+    {{{ is_pkg_init hashtriemap ∗
+        n ↦s[hashtriemap.node :: "isEntry"]□ false ∗
+        n ↦s[hashtriemap.node :: "ind"]□ i }}}
+      n @ (ptrT.id hashtriemap.node.id) @ "indirect" #()
+      {{{ RET #i; True }}}.
+  Proof.
+    wp_start as "(His_entry & Hind)".
+    wp_auto.
+    wp_finish.
+  Qed.
+
+  Lemma own_path_lookup γ q path h f :
+    h ∈ path_to_domain path →
+    own_path γ q path f -∗
+    ptsto_mut γ h q (f h) ∗ (ptsto_mut γ h q (f h) -∗ own_path γ q path f).
+  Proof.
+    iIntros (Hdom) "Hpath".
+    iDestruct (big_sepL_elem_of_acc with "Hpath") as "[Hptsto Hpath_close]"; [exact Hdom|].
+    iFrame "Hptsto Hpath_close".
+  Qed.
+
+  (* precondition: returns value, true if k is in kvs *)
+  Lemma wp_entry__lookup (ht: loc) (e: loc) (key: K) (γ: ghost_names) (path: path) :
+    ∀ (Φ: val → iProp Σ),
+    is_pkg_init hashtriemap -∗
+    "Hpre" :: (
+      "#His_map" :: is_hashtriemap γ ht ∗
+      "Hentry" :: entry γ (1/2)%Qp e path ∗
+      "Hau" :: ht_au γ (λ m, Φ (ht_load_ret m key)) ∗
+      "%Hbelongs" :: ⌜belongs_to_path path (uint.Z (hash_key key))⌝
+    ) -∗
+    WP e @ (ptrT.id hashtriemap.entry.id) @ "lookup" #key {{ Φ }}.
+  Proof.
+    intros.
+    set h := (uint.Z (hash_key key)).
+    iIntros.
+    iNamed.
+    iNamed "Hpre".
+    wp_method_call. wp_call.
+
+    wp_auto.
+
+    iAssert (
+        ∃ e,
+          "e" :: e_ptr ↦ e ∗
+          "#Hentry" :: entry γ (1 / 2) e path
+      )%I with "[$e $Hentry]" as "Hloop".
+    clear e.
+
+    wp_for "Hloop".
+
+    wp_if_destruct.
+    {
+      iApply fupd_wp.
+      iEval (rewrite entry_unfold /entry_F) in "Hentry".
+      iNamed "His_map".
+      iInv "His_map" as (rooti hm user_map) "(>? & >? & >? & #Hroot_indirect & >? & >?)" "Hclose_map".
+      iNamed.
+      iInv "Hentry_inv" as "HEI" "Hclose_entry".
+      unfold entry_inv.
+      iEval (simpl) in "HEI".
+      iMod "HEI".
+      iNamed.
+      iMod (fupd_mask_subseteq (⊤ ∖ ↑mapN ∖ ↑indN ∖ ↑entryN)) as "Hclose_au_mask"; [set_solver|].
+      iMod "Hau" as (m) "[Hown Hclose_au]".
+
+      iDestruct (ghost_var_agree with "Hown Huser_map") as %Heq.
+      subst m.
+
+      have Hdom : h ∈ path_to_domain path.
+      {
+        rewrite list_elem_of_filter.
+        split; [exact Hbelongs|].
+        apply full_domain_elem.
+      }
+
+      iDestruct (own_path_lookup _ _ _ h with "Hown_empty") as "[Hptsto Hptsto_close]"; [exact Hdom|].
+      iDestruct (map_valid with "Hauth_map Hptsto") as %Hlookup.
+      iDestruct ("Hptsto_close" with "Hptsto") as "Hown_empty".
+
+      have Hnone : user_map !! key = None.
+      {
+        rewrite Hflat.
+        rewrite (Hbuckets _ _ _ Hlookup); done.
+      }
+
+      iNamed.
+
+      iMod ("Hclose_au" with "[$]") as "HΦ".
+      iMod "Hclose_au_mask" as "_".
+      iMod ("Hclose_entry" with "[Hown_empty]") as "_"; [iNext; done|].
+      iMod ("Hclose_map" with "[$Hauth_map $Hown_root $Hroot_indirect $Hown //]") as "_".
+      iApply fupd_mask_intro; [set_solver|].
+      iIntros "_".
+      wp_alloc ret as "ret".
+      wp_auto.
+      simpl.
+      unfold ht_load_ret.
+      iEval (rewrite Hnone; simpl) in "HΦ".
+      iApply "HΦ".
+    }
+
+    iApply fupd_wp.
+    rewrite entry_unfold /entry_F.
+    iNamed.
+
+    iInv "Hentry_inv" as "HEI" "Hclose_entry".
+    unfold entry_inv.
+    destruct (decide (e = null)); [exfalso; auto|].
+    iDestruct "HEI" as (next) "(>? & HEI)".
+    iNamed.
+
+    iNamed "Hentry_step".
+
+    destruct (bool_decide (k = key)) eqn:Heq_key.
+
+    - apply bool_decide_eq_true in Heq_key.
+      replace h0 with h by (unfold h; subst; reflexivity).
+
+      iNamed "His_map".
+      iInv "His_map" as (rooti hm user_map) "(>? & >? & >? & #Hroot_indirect & >? & >?)" "Hclose_map".
+      iNamed.
+      iMod (fupd_mask_subseteq (⊤ ∖ ↑mapN ∖ ↑indN ∖ ↑entryN)) as "Hclose_au_mask"; [set_solver|].
+      iMod "Hau" as (m) "[Hown Hclose_au]".
+
+      (* linearization point *)
+
+      iDestruct (ghost_var_agree with "Hown Huser_map") as %Heq.
+      subst m.
+
+      have Hdom : h ∈ path_to_domain path.
+      {
+        rewrite list_elem_of_filter.
+        split; [exact Hbelongs|].
+        apply full_domain_elem.
+      }
+
+      iDestruct (own_path_lookup _ _ _ h with "Hown_path") as "[Hptsto Hptsto_close]"; [exact Hdom|].
+      iDestruct (map_valid with "Hauth_map Hptsto") as %Hlookup.
+      iDestruct ("Hptsto_close" with "Hptsto") as "Hown_path".
+
+      have Hsome : user_map !! key = Some v.
+      {
+        subst k.
+        rewrite Hflat.
+        rewrite (Hbuckets _ _ _ Hlookup); try done.
+        unfold singleton_map_fn.
+        rewrite decide_True; [|done].
+        rewrite lookup_insert.
+        rewrite decide_True; done.
+      }
+
+      iNamed.
+
+      iMod ("Hclose_au" with "[$]") as "HΦ".
+
+      iMod "Hclose_au_mask" as "_".
+      iMod ("Hclose_map" with "[$Hauth_map $Hown_root $Hroot_indirect $Hown //]") as "_".
+      iMod ("Hclose_entry" with "[$Hown_path $HEI]") as "_".
+      {
+        iFrame "#".
+        iPureIntro. subst k. done.
+      }
+
+      iApply fupd_mask_intro; [set_solver|].
+      iIntros "_".
+      wp_auto.
+      wp_if_destruct; [|exfalso; auto].
+
+      wp_for_post.
+
+      unfold ht_load_ret.
+
+      iEval (rewrite Hsome; simpl) in "HΦ".
+      iApply "HΦ".
+
+    - apply bool_decide_eq_false in Heq_key.
+
+      iMod ("Hclose_entry" with "[$Hown_path $HEI]") as "_"; [iFrame "#"; iPureIntro; done|].
+
+      iApply fupd_mask_intro; [set_solver|].
+      iIntros "_".
+
+      wp_auto.
+
+      wp_if_destruct; [exfalso; auto|].
+      clear Heq_key.
+      wp_apply wp_Value__Load.
+
+      iInv "Hentry_inv" as "HEI" "Hclose_entry".
+      unfold entry_inv.
+      destruct (decide (e = null)); [exfalso; auto|].
+      clear next.
+      iDestruct "HEI" as (next) "(>? & HEI)".
+      iNamed.
+
+      iApply fupd_mask_intro; [set_solver|].
+      iIntros "Hmask".
+      iNext.
+
+      iNamed "HEI".
+      iFrame "Hown_next".
+      iIntros "Hown_next".
+
+      iMod "Hmask" as "_".
+      iMod ("Hclose_entry" with "[$Hentry_step $Hown_next $Hnext_entry]") as "_".
+
+      iApply fupd_mask_intro; [set_solver|].
+      iIntros "_".
+
+      wp_apply wp_interface_type_assert; [auto|].
+
+      wp_for_post.
+      iFrame.
+      iFrame "Hnext_entry".
+  Qed.
 
   Lemma wp_hashInt (key: w64) (seed: w64) :
     {{{ is_pkg_init hashtriemap }}}
@@ -228,7 +517,7 @@ Section proof.
 
   Lemma wp_HashTrieMap__initSlow (ht: loc) (γ: ghost_names) (* P {Htimeless: ∀ m, Timeless (P m)} *) :
     {{{ is_pkg_init hashtriemap ∗ is_pkg_init atomic ∗ is_pkg_init sync ∗
-        hashtriemap_init ht γ (* P *) }}}
+        hashtriemap_init ht γ }}}
       ht @ (ptrT.id hashtriemap.HashTrieMap.id) @ "initSlow" #()
       {{{ RET #();
           hashtriemap_init ht γ (* P *) ∗ is_hashtriemap γ ht (* P *) }}}.
@@ -334,6 +623,7 @@ Section proof.
     2: { eapply into_val_typed_w64. }
 
     iIntros "Hseed".
+    iPersist "Hseed".
 
     wp_auto.
     wp_apply wp_Uint32__Store.
@@ -361,14 +651,11 @@ Section proof.
     }
 
     iMod (invariants.inv_alloc mapN _ (
-            (*                      ∃ m, *)
-            (* "HP" :: P m ∗ *)
-            "Hinv" :: ht_inv ht γ
-                               ) with "[Hhtinv]") as "#His_map".
-    { iNext. iFrame "Hhtinv". }
+              "Hinv" :: ht_inv ht γ
+            ) with "[$Hhtinv]") as "#His_map".
 
     iMod ("Hclose" with "[Htok1 Hinited His_map]") as "_".
-    { iNext. iFrame. iFrame "Hinited". iExact "His_map". }
+    { iNext. iFrame. iFrame "Hinited". unfold init_status_done. iFrame "His_map Hseed". }
     iApply fupd_mask_intro.
     {set_solver. }
     iIntros "_".
@@ -425,35 +712,26 @@ Section proof.
       + iFrame "Hinit Hmu".
         iExact "Hstatus_done".
       + exfalso. congruence.
-    Qed.
+  Qed.
 
   (* dont actually need the is_hashtriemap precondition for any of the lemmas because initHT gives it to us *)
-  (* Lemma wp_HashTrieMap__Load (ht: loc) (key: w64) (γ: ghost_names) P Q *)
-  (*       {Htimeless: ∀ m, Timeless (P m)} : *)
-  (*   {{{ is_pkg_init hashtriemap ∗ is_pkg_init atomic ∗ is_pkg_init sync ∗ *)
-  (*       hashtriemap_init ht γ P ∗ is_hashtriemap γ ht P ∗ *)
-  (*       (∀ m, P m -∗ |==> P m ∗ Q (map_get (m !! key))) *)
-  (*   }}} *)
-  (*     ht @ (ptrT.id hashtriemap.HashTrieMap.id) @ "Load" #key *)
-  (*     {{{ (v: w64) (ok: bool), RET (#v, #ok); Q (v, ok) }}}. *)
-  (* Proof. *)
   Lemma wp_HashTrieMap__Load (ht: loc) (key: w64) (γ: ghost_names) :
-    {{{ is_pkg_init hashtriemap ∗ is_pkg_init atomic ∗ is_pkg_init sync ∗
-        hashtriemap_init ht γ
-    }}}
-      ht @ (ptrT.id hashtriemap.HashTrieMap.id) @ "Load" #key
-      {{{ (v: w64) (ok: bool), RET (#v, #ok); True }}}.
+    ∀ (Φ: val → iProp Σ),
+    (is_pkg_init hashtriemap ∗ is_pkg_init atomic ∗ is_pkg_init sync ∗
+     "Hinit" :: hashtriemap_init ht γ ∗
+     "Hau" :: ht_au γ (λ m, Φ (ht_load_ret m key))) -∗
+    WP ht @ (ptrT.id hashtriemap.HashTrieMap.id) @ "Load" #key {{ Φ }}.
   Proof.
-    wp_start as "Hpre".
+    iIntros (Φ) "(#? & #? & #? & Hpre)".
     iNamed "Hpre".
+
+    wp_method_call. wp_call.
 
     wp_auto.
 
     wp_apply (wp_HashTrieMap__initHT with "[$]").
-    iIntros "(_ & #His_map)".
-    wp_auto.
-
-    iApply struct_fields_split in "ht".
+    iIntros "(_ & His_map)".
+    iNamed "His_map".
     wp_auto.
 
     wp_apply wp_hashInt.
@@ -461,56 +739,58 @@ Section proof.
 
     wp_auto.
 
-    iApply struct_fields_split in "ht".
-    wp_auto.
     wp_apply wp_Value__Load.
     iInv "His_map" as "Hhtinv" "Hclose".
-
     iApply fupd_mask_intro.
     { set_solver. }
     iIntros "Hmask".
     iNext.
     iNamed "Hhtinv".
+    iEval (unfold ht_inv) in "Hinv".
     iNamed "Hinv".
     iFrame "Hown_root".
     iIntros "Hown_root".
     iMod "Hmask".
-    iMod ("Hclose" with "[$]").
     iClear "Hmask".
+
+    unfold ht_inv.
+    iMod ("Hclose" with "[$Hauth_map $Huser_map $Hown_root $Hroot_indirect]") as "_"; [iNext; iPureIntro; done|].
+
     iApply fupd_mask_intro.
     { set_solver. }
     iIntros "_".
-    wp_auto.
+
+    clear Hflat.
+    clear Hbuckets.
+    clear hm. clear user_map.
 
     wp_apply wp_interface_type_assert.
     { auto. }
 
+    set h := uint.Z (hash_key key).
+
     iAssert (∃ (path: path) (shift: w64) (cur: loc),
                 "Hcur" :: i_ptr ↦ cur ∗
-                "%Hpathlen" :: ⌜length path < 16⌝ ∗
-                "#Hi_indirect" :: indirect γ cur path ∗
                 "Hhash_shift" :: hashShift_ptr ↦ shift ∗
-                "%Hshift" :: ⌜shift = sh path⌝
-            (* TODO: add pure condition that *)
-            (*
-(w64_word_instance.(word.and)
-                                 (w64_word_instance.(word.sru) 
-                                    (hash_key key)
-                                    (w64_word_instance.(word.sub) 
-                                       (W64 (sh path))
-                                       (W64 hashtriemap.nChildrenLog2)))
-                                 (W64 hashtriemap.nChildrenMask))
-                                 is next nibble on path to hash_key key
-             *)
+                "#Hi_indirect" :: indirect γ cur path ∗
+                "%Hshift" :: ⌜shift = sh path⌝ ∗
+                "%Hpath_len" :: ⌜length path < 16⌝ ∗
+                "%Hkey_path" :: ⌜belongs_to_path path h⌝
             )%I with ("[$Hroot_indirect $hashShift $i]") as "Hloop_inv".
-    { iSplit; eauto. }
+    {
+      repeat iSplit; eauto.
+      iPureIntro.
+      unfold belongs_to_path, sh, path_to_prefix.
+      simpl.
+      rewrite Z.shiftr_div_pow2; try word.
+    }
+    iClear "Hroot_indirect".
 
     wp_for "Hloop_inv".
 
-    iClear "Hroot_indirect".
-    rewrite indirect_unfold /indirect_F.
+    iEval (rewrite indirect_unfold /indirect_F) in "Hi_indirect".
     iNamed "Hi_indirect".
-    
+
     wp_if_destruct.
     {
       wp_apply wp_panic.
@@ -520,14 +800,14 @@ Section proof.
     }
 
     iDestruct (own_slice_len with "Hchildren_slice") as "(%Hlen_children_16 & _)".
-    have Hlen_children : sint.Z children_slice.(slice.len_f) = 16.
+    have Hlen_children : uint.Z children_slice.(slice.len_f) = 16.
     { word. }
     clear Hlen_children_16.
 
+    unfold hashtriemap.nChildrenLog2, hashtriemap.nChildrenMask in *.
     wp_pure.
     {
-      unfold hashtriemap.nChildrenLog2, hashtriemap.nChildrenMask.
-      have Hlen16 : sint.Z children_slice.(slice.len_f) = 16 by word.
+      have Hlen16 : uint.Z children_slice.(slice.len_f) = 16 by word.
       set (x := w64_word_instance.(word.sru) (hash_key key)
                                     (w64_word_instance.(word.sub) (W64 (64 - 4 * length path)) (W64 4))).
       have Hnib_u : 0 ≤ uint.Z (w64_word_instance.(word.and) x (W64 15)) < 16.
@@ -545,16 +825,14 @@ Section proof.
       word.
     }
 
-    unfold hashtriemap.nChildrenMask.
-    unfold hashtriemap.nChildrenLog2.
     set next_nibble := (w64_word_instance.(word.and)
                                             (w64_word_instance.(word.sru)
                                                                  (hash_key key)
                                                                  (w64_word_instance.(word.sub)
-                                                                                      (W64 (sh path)) 
+                                                                                      (W64 (sh path))
                                                                                       (W64 4)))
                                             (W64 15)).
-    
+
     have Hnib_u : 0 ≤ uint.Z next_nibble < 16.
     {
       unfold next_nibble.
@@ -576,11 +854,26 @@ Section proof.
     destruct (lookup_lt_is_Some_2 children_vals (sint.nat next_nibble) Hlt_nat)
       as [v Hv].
 
-    wp_pures.
+    wp_auto.
+
+    have Hdom : h ∈ path_to_domain path.
+    {
+      unfold path_to_domain.
+      rewrite list_elem_of_filter.
+      split.
+      - exact Hkey_path.
+      - apply full_domain_elem.
+    }
+
+    unfold ht_au.
     wp_apply wp_Value__Load.
+    iInv "His_map" as "Hhtinv" "Hclose_ht".
     iInv "Hind_inv" as "HI" "Hclose_ind".
+
+    unfold own_ht_map.
     iApply fupd_mask_intro.
-    { set_solver. }
+    { apply empty_subseteq.
+    (* set_solver. doesnt work, only when Hdom is defined? *) }
     iIntros "Hmask".
     iNext.
 
@@ -588,20 +881,166 @@ Section proof.
 
     iNamed "HI".
 
+    iNamed "Hhtinv".
+    iNamed "Hinv".
+
     iDestruct (big_sepL_lookup_acc with "Hchildren") as "[Hchild Hchildren_close]".
     { exact Hv. }
     iNamed "Hchild".
     iExists (interface.mk (ptrT.id hashtriemap.node.id) (# nodeptr)).
-
     replace (W64 (sint.nat next_nibble)) with next_nibble by word.
     iFrame "Hown_child".
     iIntros "Hown_child".
-    iDestruct ("Hchildren_close" with "[Hown_child Hchild]") as "Hchildren".
-    { iExists nodeptr. iFrame. }
+
+    unfold ht_load_ret.
+    iEval (unfold childP) in "Hchild".
+
+    unfold own_path.
+
+    destruct (decide (nodeptr = null)).
+    {
+      iMod "Hmask" as "_".
+
+      iMod (fupd_mask_subseteq ht_au_mask) as "Hclose_au_mask".
+      {
+        unfold ht_au_mask.
+        apply subseteq_difference_l.
+        set_solver.
+      }
+
+      iMod "Hau" as (m) "[Hown Hclose_au]". (* linearization point *)
+      iDestruct (ghost_var_agree with "Huser_map Hown") as %meq.
+      subst m.
+
+      iDestruct (big_sepL_elem_of_acc with "Hchild") as "[Hptsto Hptsto_close]".
+      { exact Hdom. }
+      iDestruct (map_valid with "Hauth_map Hptsto") as %Hlookup.
+      iDestruct ("Hptsto_close" with "Hptsto") as "Hchild".
+
+      iDestruct ("Hchildren_close" with "[Hown_child Hchild]") as "Hchildren".
+      { iExists nodeptr. iFrame. unfold childP.
+        destruct (decide (nodeptr = null)).
+        - iFrame.
+        - contradiction n0.
+      }
+
+      iMod ("Hclose_au" with "Hown") as "HΦ".
+      iMod "Hclose_au_mask" as "_".
+      iMod ("Hclose_ind" with "Hchildren") as "_".
+      iMod ("Hclose_ht" with "[$Hauth_map $Hown_root $Hroot_indirect $Huser_map //]") as "_".
+
+      iApply fupd_mask_intro.
+      { set_solver. }
+      iIntros "_".
+
+      wp_apply wp_interface_type_assert.
+      { auto. }
+
+      wp_bind.
+      replace (bool_decide (nodeptr = null)) with true.
+      2: { symmetry. rewrite (bool_decide_eq_true (nodeptr = null)). exact e. }
+
+      wp_auto.
+      wp_bind.
+      wp_alloc d_ptr as "d_ptr".
+      wp_auto.
+      wp_for_post.
+
+      have Hnone : (user_map !! key = None).
+      {
+        subst user_map.
+        unfold empty_map_fn in Hlookup.
+        have Hflat : flatten hm !! key = (∅ : gmap K V) !! key.
+        { apply (Hbuckets h ∅ key); [exact Hlookup|reflexivity]. }
+        rewrite Hflat.
+        rewrite lookup_empty.
+        done.
+      }
+      iEval (rewrite Hnone; simpl) in "HΦ".
+      iApply "HΦ".
+    }
+
+    iDestruct "Hchild" as (is_entry) "(#Hnodeis_entry & #Hchild)".
+    destruct is_entry.
+    {
+      iDestruct "Hchild" as (ent) "(#Hent & #Hind_null & #Hentry)".
+      iMod "Hmask" as "_".
+
+      iEval (rewrite entry_unfold /entry_F) in "Hentry".
+      iNamed "Hentry".
+
+      iMod (fupd_mask_subseteq ht_au_mask) as "Hclose_au_mask".
+      {
+        unfold ht_au_mask.
+        apply subseteq_difference_l.
+        set_solver.
+      }
+
+      iDestruct ("Hchildren_close" with "[Hown_child]") as "Hchildren".
+      { iExists nodeptr. iFrame. unfold childP.
+        destruct (decide (nodeptr = null)).
+        - contradiction n0.
+        - iExists true. iFrame "#". rewrite entry_unfold /entry_F. iFrame "#".
+      }
+
+      iMod "Hclose_au_mask" as "_".
+      iMod ("Hclose_ind" with "[$Hchildren]") as "_".
+      iMod ("Hclose_ht" with "[$Hauth_map $Hown_root $Hroot_indirect $Huser_map //]") as "_".
+
+      iApply fupd_mask_intro.
+      { set_solver. }
+      iIntros "_".
+
+      wp_apply wp_interface_type_assert.
+      { auto. }
+      replace (bool_decide (nodeptr = null)) with false.
+      2: { symmetry. rewrite (bool_decide_eq_false (nodeptr = null)). exact n0. }
+
+      wp_auto.
+
+      wp_apply wp_node__entry; [iFrame "Hnodeis_entry Hent"|].
+      wp_apply wp_entry__lookup.
+      iFrame "His_map Hseed".
+      rewrite /named.
+      repeat iSplit; eauto.
+      {
+        rewrite entry_unfold /entry_F.
+        iFrame "Hentry_inv".
+      }
+      unfold ht_au.
+      iMod "Hau".
+      iApply fupd_mask_intro.
+      { apply empty_subseteq. }
+
+      iIntros "_".
+      iDestruct "Hau" as (m) "[Huser_own Hclose_au]".
+      iFrame "Huser_own".
+      iIntros "Huser_own".
+
+      iDestruct ("Hclose_au" with "Huser_own") as "Hau".
+      iMod "Hau".
+
+      iApply fupd_mask_intro.
+      { set_solver. }
+      iIntros "_".
+
+      wp_auto.
+      wp_for_post.
+      iFrame.
+    }
+    iDestruct "Hchild" as (ind) "(%Hnext_path_len & #Hent_null & #Hind & #Hindirect)".
+
+    iDestruct ("Hchildren_close" with "[Hown_child]") as "Hchildren".
+    { iExists nodeptr. iFrame. unfold childP.
+      destruct (decide (nodeptr = null)).
+      - contradiction n0.
+      - iExists false. iFrame "#".
+        iPureIntro. exact Hnext_path_len.
+    }
 
     iMod "Hmask" as "_".
-
     iMod ("Hclose_ind" with "Hchildren") as "_".
+    iMod ("Hclose_ht" with "[$Hauth_map $Hown_root $Hroot_indirect $Huser_map //]") as "_".
 
     iApply fupd_mask_intro.
     { set_solver. }
@@ -610,19 +1049,40 @@ Section proof.
     wp_apply wp_interface_type_assert.
     { auto. }
 
-    wp_if_destruct.
-    {
-      wp_bind.
-      wp_alloc d_ptr as "d_ptr".
-      wp_auto.
-      wp_for_post.
-      admit.
-      (* wp_finish *)
-      (* need to figure out specs *)
-    }
-    iApply struct_fields_split in "n".
+    replace (bool_decide (nodeptr = null)) with false.
+    2: { symmetry. rewrite (bool_decide_eq_false (nodeptr = null)). exact n0. }
+
     wp_auto.
-  Admitted.
+    wp_apply (wp_node__indirect with "[$]").
+    wp_for_post.
+    iFrame.
+    iFrame "#".
+    iPureIntro.
+
+    set next := Z.of_nat (sint.nat next_nibble).
+    set next_path := (path ++ [next]).
+
+    have Hlen : length next_path = (length path + 1)%nat by
+                                         rewrite app_length /=.
+
+    have Hz : uint.Z next_nibble = Z.land (h ≫ (sh path - 4)) 15.
+    {
+      rewrite next_nibble_eq.
+      - reflexivity.
+      - auto.
+    }
+
+    split_and!; auto.
+    - rewrite sh_snoc. unfold sh. word.
+    - apply (next_nibble_extend path h next); try done.
+      + unfold h.
+        pose proof (word.unsigned_range (hash_key key)) as [H0 _].
+        exact H0.
+      + unfold next.
+        rewrite Z2Nat.id; [|word].
+        rewrite <- Z2Nat.id with (n:=sint.Z next_nibble) by word.
+        word.
+  Qed.
 
   Lemma wp_HashTrieMap__LoadOrStore (ht: loc) (key: w64) (value: w64) :
     {{{ is_pkg_init hashtriemap }}}
@@ -714,12 +1174,6 @@ Section proof.
       {{{ (a: loc), RET (#a); True }}}.
   Proof. Admitted.
 
-  Lemma wp_entry__lookup (e: loc) (key: w64) :
-    {{{ is_pkg_init hashtriemap }}}
-      e @ (ptrT.id hashtriemap.entry.id) @ "lookup" #key
-      {{{ (a: w64) (b: bool), RET (#a, #b); True }}}.
-  Proof. Admitted.
-
   Lemma wp_entry__lookupWithValue (e: loc) (key: w64) (value: w64) (checkValue: bool) :
     {{{ is_pkg_init hashtriemap }}}
       e @ (ptrT.id hashtriemap.entry.id) @ "lookupWithValue" #key #value #checkValue
@@ -748,18 +1202,6 @@ Section proof.
     {{{ is_pkg_init hashtriemap }}}
       head @ (ptrT.id hashtriemap.entry.id) @ "compareAndDelete" #key #value
       {{{ (a: loc) (b: bool), RET (#a, #b); True }}}.
-  Proof. Admitted.
-
-  Lemma wp_node__entry (n: loc) :
-    {{{ is_pkg_init hashtriemap }}}
-      n @ (ptrT.id hashtriemap.node.id) @ "entry" #()
-      {{{ (a: loc), RET (#a); True }}}.
-  Proof. Admitted.
-
-  Lemma wp_node__indirect (n: loc) :
-    {{{ is_pkg_init hashtriemap }}}
-      n @ (ptrT.id hashtriemap.node.id) @ "indirect" #()
-      {{{ (a: loc), RET (#a); True }}}.
   Proof. Admitted.
 
 End proof.
